fix
git-svn-id: svn://scm.gforge.inria.fr/svn/cfml@341 ba02c806-7d2b-4818-9a48-35b22e6bdc79

imper/Dijkstra.ml
@@ -32,25 +32,25 @@ sig
   val pop : heap -> NextNode.t
 end
 
-module Dijkstra (Heap:HeapNextNodeSig) = (* Heap : HeapSig with module Element = NextNode *)
+module Dijkstra (Pqueue:HeapNextNodeSig) = (* Heap : HeapSig with module Element = NextNode *)
 struct 
    let shortest_path g s e = 
       let n = Array.length g in
       let b = Array.make n Infinite in
       let v = Array.make n false in
-      let h = Heap.create() in
+      let q = Pqueue.create() in
       b.(s) <- Finite 0;
-      Heap.push (s,0) h;
-      while not (Heap.is_empty h) do
-         let (x,dx) = Heap.pop h in
+      Pqueue.push (s,0) q;
+      while not (Pqueue.is_empty q) do
+         let (x,dx) = Pqueue.pop q in
          if not v.(x) then begin
             v.(x) <- true;
             let update (y,w) =
-              let dy = dx + w in
-                 if (match b.(y) with | Finite d -> dy < d
-                                      | _ -> true) then 
-                    (b.(y) <- Finite dy; 
-                     Heap.push (y,dy) h)
+               let dy = dx + w in
+               if (match b.(y) with | Finite d -> dy < d
+                                    | Infinite -> true)  
+                  then (b.(y) <- Finite dy; 
+                        Pqueue.push (y,dy) q)
                in
             List.iter update g.(x);
          end;
